src/cddl/pulse/CDDL.Pulse.Parse.MapGroup.fst
@@ -1,0 +1,303 @@
+module CDDL.Pulse.Parse.MapGroup
+include CDDL.Pulse.MapGroup
+include CDDL.Pulse.Parse.Base
+open Pulse.Lib.Pervasives
+open CBOR.Spec.API.Type
+open CBOR.Pulse.API.Base
+module Trade = Pulse.Lib.Trade.Util
+module R = Pulse.Lib.Reference
+module U64 = FStar.UInt64
+
+let impl_zero_copy_map_group_pre
+  (g: det_map_group)
+  (f: typ)
+  (v: cbor)
+  (m1 m2: cbor_map)
+: Tot prop
+=
+  map_group_parser_spec_arg_prop g f m1 /\
+  cbor_map_disjoint m1 m2 /\
+  cbor_map_disjoint_from_footprint m2 f /\
+  begin match unpack v with
+  | CMap m ->
+    cbor_map_equal m (cbor_map_union m1 m2)
+  | _ -> False
+  end
+
+let impl_zero_copy_map_group_post
+  (#tgt: Type0)
+  (#tgt_size: tgt -> nat)
+  (#tgt_prop: tgt -> bool)
+  (#g: det_map_group)
+  (#f: typ)
+  (ps: map_group_parser_spec g f tgt_size tgt_prop)
+  (v: cbor)
+  (m1 m2: cbor_map)
+  (v': tgt)
+: Tot prop
+=
+  impl_zero_copy_map_group_pre g f v m1 m2 /\
+  (ps m1 <: tgt) == v'
+
+inline_for_extraction
+let impl_zero_copy_map_group
+  (#t: Type0)
+  (vmatch: perm -> t -> cbor -> slprop)
+  (#g: det_map_group)
+  (#f: typ)
+  (#tgt: Type0)
+  (#tgt_size: tgt -> nat)
+  (#tgt_prop: tgt -> bool)
+  (ps: map_group_parser_spec g f tgt_size tgt_prop)
+  (#impl_tgt: Type0)
+  (r: rel impl_tgt tgt)
+=
+  (c: t) ->
+  (#p: perm) ->
+  (#v: Ghost.erased cbor) ->
+  (v1: Ghost.erased cbor_map) ->
+  (v2: Ghost.erased cbor_map) ->
+  stt impl_tgt
+        (
+          vmatch p c v **
+          pure (impl_zero_copy_map_group_pre g f v v1 v2)
+        )
+        (fun res -> exists* v' .
+          r res v' **
+          Trade.trade (r res v') (vmatch p c v) **
+          pure (impl_zero_copy_map_group_post ps v v1 v2 v')
+        )
+
+module Util = CBOR.Spec.Util
+
+inline_for_extraction noextract [@@noextract_to "krml"]
+```pulse
+fn impl_zero_copy_map
+  (#ty: Type0)
+  (#vmatch: perm -> ty -> cbor -> slprop)
+    (#t: Ghost.erased (det_map_group))
+    (#fp: Ghost.erased typ)
+    (#tgt: Type0)
+    (#tgt_size: Ghost.erased (tgt -> nat))
+    (#tgt_serializable: Ghost.erased (tgt -> bool))
+    (#ps: Ghost.erased (map_group_parser_spec t fp tgt_size tgt_serializable))
+    (#impl_tgt: Type0)
+    (#r: rel impl_tgt tgt)
+    (pa: impl_zero_copy_map_group vmatch ps r)
+    (sq: squash (
+      map_group_footprint t fp
+    ))
+: impl_zero_copy_parse #ty vmatch #(t_map (Ghost.reveal t)) #tgt #(spec_map_group_serializable (Ghost.reveal tgt_size) (Ghost.reveal tgt_serializable)) (parser_spec_map_group (Ghost.reveal t) (Ghost.reveal ps) (spec_map_group_serializable (Ghost.reveal tgt_size) (Ghost.reveal tgt_serializable))) #impl_tgt r
+=
+  (c: _)
+  (#p: _)
+  (#v: _)
+{
+  let m : Ghost.erased cbor_map = Ghost.hide (CMap?.c (unpack v));
+  let m1 : Ghost.erased cbor_map = Ghost.hide (cbor_map_filter (matches_map_group_entry fp any) m);
+  let m2 : Ghost.erased cbor_map = Ghost.hide (cbor_map_filter (Util.notp (matches_map_group_entry fp any)) m);
+  parser_spec_map_group_eq t ps (spec_map_group_serializable (Ghost.reveal tgt_size) (Ghost.reveal tgt_serializable)) v; // FIXME: WHY WHY WHY does the pattern not trigger?
+  pa c m1 m2
+}
+```
+
+let rel_either_eq_left
+  (#low1 #high1: Type)
+  (r1: rel low1 high1)
+  (#low2 #high2: Type)
+  (r2: rel low2 high2)
+  (w1: low1)
+  (z1: high1)
+: Lemma
+  (rel_either r1 r2 (Inl w1) (Inl z1) == r1 w1 z1)
+= ()
+
+let rel_either_eq_right
+  (#low1 #high1: Type)
+  (r1: rel low1 high1)
+  (#low2 #high2: Type)
+  (r2: rel low2 high2)
+  (w2: low2)
+  (z2: high2)
+: Lemma
+  (rel_either r1 r2 (Inr w2) (Inr z2) == r2 w2 z2)
+= ()
+
+#set-options "--print_implicits"
+
+#push-options "--ifuel 8"
+
+#restart-solver
+
+inline_for_extraction noextract [@@noextract_to "krml"]
+```pulse
+fn impl_zero_copy_map_choice
+  (#ty: Type0)
+  (#vmatch: perm -> ty -> cbor -> slprop)
+    (#t1: Ghost.erased (det_map_group))
+    (#fp1: Ghost.erased typ)
+    (#tgt1: Type0)
+    (#tgt_size1: Ghost.erased (tgt1 -> nat))
+    (#tgt_serializable1: Ghost.erased (tgt1 -> bool))
+    (#ps1: Ghost.erased (map_group_parser_spec t1 fp1 tgt_size1 tgt_serializable1))
+    (#impl_tgt1: Type0)
+    (#r1: rel impl_tgt1 tgt1)
+    (va1: impl_map_group_t vmatch t1 fp1)
+    (pa1: impl_zero_copy_map_group vmatch ps1 r1)
+    (#t2: Ghost.erased (det_map_group))
+    (#fp2: Ghost.erased typ)
+    (#tgt2: Type0)
+    (#tgt_size2: Ghost.erased (tgt2 -> nat))
+    (#tgt_serializable2: Ghost.erased (tgt2 -> bool))
+    (#ps2: Ghost.erased (map_group_parser_spec t2 fp2 tgt_size2 tgt_serializable2))
+    (#impl_tgt2: Type0)
+    (#r2: rel impl_tgt2 tgt2)
+    (pa2: impl_zero_copy_map_group vmatch ps2 r2)
+    (sq: squash (
+      map_group_footprint t1 fp1 /\
+      map_group_footprint t2 fp2
+    ))
+: impl_zero_copy_map_group #ty vmatch #(map_group_choice (Ghost.reveal t1) (Ghost.reveal t2)) #(t_choice (Ghost.reveal fp1) (Ghost.reveal fp2))
+#(either tgt1 tgt2) #(mg_spec_choice_size (Ghost.reveal tgt_size1) (Ghost.reveal tgt_size2)) #(mg_spec_choice_serializable (Ghost.reveal tgt_serializable1) (Ghost.reveal tgt_serializable2)) (map_group_parser_spec_choice (Ghost.reveal ps1) (Ghost.reveal ps2) (mg_spec_choice_size (Ghost.reveal tgt_size1) (Ghost.reveal tgt_size2)) (mg_spec_choice_serializable (Ghost.reveal tgt_serializable1) (Ghost.reveal tgt_serializable2))) #(either impl_tgt1 impl_tgt2) (rel_either r1 r2)
+=
+  (c: _)
+  (#p: _)
+  (#v: _)
+  (v1: _)
+  (v2: _)
+{
+  map_group_footprint_choice t1 t2 fp1 fp2;
+  map_group_parser_spec_choice_eq (Ghost.reveal ps1) (Ghost.reveal ps2) (mg_spec_choice_size (Ghost.reveal tgt_size1) (Ghost.reveal tgt_size2)) (mg_spec_choice_serializable (Ghost.reveal tgt_serializable1) (Ghost.reveal tgt_serializable2)) v1;
+  let mut dummy = 0uL;
+  let m1 = Ghost.hide (cbor_map_filter (matches_map_group_entry fp1 any) v1);
+  let cm1 = Ghost.hide (cbor_map_sub v1 m1);
+  let v21 = Ghost.hide (cbor_map_union cm1 v2);
+  let test1 = va1 c m1 v21 false dummy;
+  if (MGOK? test1) {
+    let w1 = pa1 c m1 v21;
+    with z1 . assert (r1 w1 z1);
+    let res : either impl_tgt1 impl_tgt2 = Inl w1;
+    rel_either_eq_left r1 r2 w1 z1;
+    Trade.rewrite_with_trade (r1 w1 z1) (rel_either r1 r2 res (Inl z1));
+    Trade.trans _ _ (vmatch p c v);
+    res
+  } else {
+    let m2 = Ghost.hide (cbor_map_filter (matches_map_group_entry fp2 any) v1);
+    let cm2 = Ghost.hide (cbor_map_sub v1 m2);
+    let v22 = Ghost.hide (cbor_map_union cm2 v2);
+    // FIXME: WHY WHY WHY those asserts?
+    assert (pure (map_group_parser_spec_arg_prop t2 fp2 m2));
+    assert (pure (cbor_map_disjoint m2 v22));
+    assert (pure (cbor_map_disjoint_from_footprint v22 fp2));
+    assert (pure (cbor_map_equal (cbor_map_union v1 v2) (cbor_map_union m2 v22)));
+    let w2 = pa2 c m2 v22;
+    with z2 . assert (r2 w2 z2);
+    let res : either impl_tgt1 impl_tgt2 = Inr w2;
+    rel_either_eq_right r1 r2 w2 z2;
+    Trade.rewrite_with_trade (r2 w2 z2) (rel_either r1 r2 res (Inr z2));
+    Trade.trans _ _ (vmatch p c v);
+    res
+  }
+}
+```
+
+let rel_pair_eq
+  (#low1 #high1: Type)
+  (r1: rel low1 high1)
+  (#low2 #high2: Type)
+  (r2: rel low2 high2)
+  (w1: low1)
+  (w2: low2)
+  (z1: high1)
+  (z2: high2)
+: Lemma
+  (rel_pair r1 r2 (w1, w2) (z1, z2) == r1 w1 z1 ** r2 w2 z2)
+= ()
+
+#restart-solver
+
+inline_for_extraction noextract [@@noextract_to "krml"]
+```pulse
+fn impl_zero_copy_map_concat
+  (#ty: Type0)
+  (#vmatch: perm -> ty -> cbor -> slprop)
+  (share: share_t vmatch)
+  (gather: gather_t vmatch)
+    (#t1: Ghost.erased (det_map_group))
+    (#fp1: Ghost.erased typ)
+    (#tgt1: Type0)
+    (#tgt_size1: Ghost.erased (tgt1 -> nat))
+    (#tgt_serializable1: Ghost.erased (tgt1 -> bool))
+    (#ps1: Ghost.erased (map_group_parser_spec t1 fp1 tgt_size1 tgt_serializable1))
+    (#impl_tgt1: Type0)
+    (#r1: rel impl_tgt1 tgt1)
+    (pa1: impl_zero_copy_map_group vmatch ps1 r1)
+    (#t2: Ghost.erased (det_map_group))
+    (#fp2: Ghost.erased typ)
+    (#tgt2: Type0)
+    (#tgt_size2: Ghost.erased (tgt2 -> nat))
+    (#tgt_serializable2: Ghost.erased (tgt2 -> bool))
+    (#ps2: Ghost.erased (map_group_parser_spec t2 fp2 tgt_size2 tgt_serializable2))
+    (#impl_tgt2: Type0)
+    (#r2: rel impl_tgt2 tgt2)
+    (pa2: impl_zero_copy_map_group vmatch ps2 r2)
+    (sq: squash (
+      map_group_footprint t1 fp1 /\
+      map_group_footprint t2 fp2 /\
+      typ_disjoint fp1 fp2
+    ))
+: impl_zero_copy_map_group #ty vmatch #(map_group_concat (Ghost.reveal t1) (Ghost.reveal t2)) #(t_choice (Ghost.reveal fp1) (Ghost.reveal fp2))
+#(tgt1 & tgt2) #(mg_spec_concat_size (Ghost.reveal tgt_size1) (Ghost.reveal tgt_size2)) #(mg_spec_concat_serializable (Ghost.reveal tgt_serializable1) (Ghost.reveal tgt_serializable2)) (map_group_parser_spec_concat (Ghost.reveal ps1) (Ghost.reveal ps2) (mg_spec_concat_size (Ghost.reveal tgt_size1) (Ghost.reveal tgt_size2)) (mg_spec_concat_serializable (Ghost.reveal tgt_serializable1) (Ghost.reveal tgt_serializable2))) #(impl_tgt1 & impl_tgt2) (rel_pair r1 r2)
+=
+  (c: _)
+  (#p: _)
+  (#v: _)
+  (v1: _)
+  (v2: _)
+{
+  map_group_footprint_concat t1 t2 fp1 fp2;
+  map_group_parser_spec_concat_eq (Ghost.reveal ps1) (Ghost.reveal ps2) (mg_spec_concat_size (Ghost.reveal tgt_size1) (Ghost.reveal tgt_size2)) (mg_spec_concat_serializable (Ghost.reveal tgt_serializable1) (Ghost.reveal tgt_serializable2)) v1;
+  share c;
+  ghost fn aux (_: unit)
+  requires emp ** (vmatch (p /. 2.0R) c v ** vmatch (p /. 2.0R) c v)
+  ensures vmatch p c v
+  {
+    gather c #(p /. 2.0R) #v #(p /. 2.0R) #v;
+    rewrite (vmatch (p /. 2.0R +. p /. 2.0R) c v)
+      as (vmatch p c v)
+  };
+  Trade.intro _ _ _ aux;
+  let m1 = Ghost.hide (cbor_map_filter (matches_map_group_entry fp1 any) v1);
+  let cm1 = Ghost.hide (cbor_map_sub v1 m1);
+  let v21 = Ghost.hide (cbor_map_union cm1 v2);
+  // FIXME: WHY WHY WHY those asserts?
+  assert (pure (map_group_parser_spec_arg_prop t1 fp1 m1));
+  assert (pure (cbor_map_disjoint m1 v21));
+  assert (pure (cbor_map_disjoint_from_footprint v21 fp1));
+  assert (pure (cbor_map_equal (cbor_map_union v1 v2) (cbor_map_union m1 v21)));
+  let w1 = pa1 c m1 v21;
+  with z1 . assert (r1 w1 z1);
+  Trade.trans_hyp_l _ _ _ _;
+  let m2 = Ghost.hide (cbor_map_filter (matches_map_group_entry fp2 any) v1);
+  let cm2 = Ghost.hide (cbor_map_sub v1 m2);
+  let v22 = Ghost.hide (cbor_map_union cm2 v2);
+  // FIXME: WHY WHY WHY those asserts?
+  assert (pure (map_group_parser_spec_arg_prop t2 fp2 m2));
+  assert (pure (cbor_map_disjoint m2 v22));
+  assert (pure (cbor_map_disjoint_from_footprint v22 fp2));
+  assert (pure (cbor_map_equal (cbor_map_union v1 v2) (cbor_map_union m2 v22)));
+  let w2 = pa2 c m2 v22;
+  with z2 . assert (r2 w2 z2);
+  Trade.trans_hyp_r _ _ _ _;
+  let res = (w1, w2);
+  rel_pair_eq r1 r2 w1 w2 z1 z2;
+  Trade.rewrite_with_trade
+    (r1 w1 z1 ** r2 w2 z2)
+    (rel_pair r1 r2 res (z1, z2));
+  Trade.trans _ _ (vmatch p c v);
+  res
+}
+```
+
+#pop-options
+
